inductive invariants

working/composition/event_based_refinement/load_balancer/service_correspondence/addition_service/AdditionServiceSM.t.dfy
@@ -1,25 +1,22 @@
-include "../shared/AbstractServiceSpec.t.dfy"
+include "../shared/AbstractServiceSM.t.dfy"
 
-module AdditionServiceSpec refines AbstractServiceSpec {
+module AdditionServiceSM refines AbstractServiceSM {
     
     datatype Constants = Constants(idSelf: ClientId)
 
     datatype ServiceRequest = AddRequest(seqNo: nat, x: int, y: int)
     datatype ServiceReply = AddReply(seqNo: nat, sum: int)
 
-    datatype Variables = Variables(requests: set<Message<ServiceRequest>>, replies: set<Message<ServiceReply>>)
+    datatype Variables = Variables()
 
     ghost predicate Init(c: Constants, v: Variables) {
-        && |v.requests| == 0
-        && |v.replies| == 0
+        true
     }
 
     ghost predicate Add(c: Constants, v: Variables, v': Variables, msgOps: MessageOps) {
         exists request : Message<ServiceRequest>, reply : Message<ServiceReply> ::
             && msgOps.recv == {Message(request.src, request.dest, MarshallServiceRequest(request.msg))} 
             && msgOps.send == {Message(reply.src, reply.dest, MarshallServiceReply(reply.msg))}
-            && v'.requests == v.requests + {request}
-            && v'.replies == v.replies + {reply}
             && reply.msg == AddReply(request.msg.seqNo, request.msg.x + request.msg.y)
             && reply.dest == request.src
     }
