working/composition/event_based_refinement/load_balancer/service_correspondence/multiplication_service/RefinementProof.v.dfy
@@ -1,89 +1,324 @@
 include "RefinementObligation.t.dfy"
 
 module RefinementProof refines RefinementTheorem {
-    ghost function ConstantsAbstraction(c: Constants) : Spec.Constants
+    ghost function ConstantsAbstraction(c: Constants) : Service.Constants
         //requires c.WF()
     {
-        Spec.Constants
+        Service.Constants
     }
 
-    ghost function VariablesAbstraction(c: Constants, v: Variables) : Spec.Variables
+    ghost function VariablesAbstraction(c: Constants, v: Variables) : Service.Variables
         //requires v.WF(c)
     {
-        Spec.Variables(v.multSvc.hosts[0].requests, v.multSvc.hosts[0].replies)
+        Service.Variables(v.multSvc.hosts[0].requests, v.multSvc.hosts[0].replies)
     }
 
-    // todo -- generalize these invariants and bake them into the system model?
-    ghost predicate Inv_AddSvcCorrespondence(c: Constants, v: Variables)
-        requires v.WF(c)
-    {
-        && (forall pkt: Message<seq<byte>> :: 
-            && pkt in v.network.sentMsgs
-            && AddSvc.ParseServiceReply(pkt.msg).Some? ==>
-                exists request: Message<AddSvc.ServiceRequest> :: 
-                && Message(pkt.src, pkt.dest, AddSvc.ParseServiceReply(pkt.msg).value) in v.addSvc.replies
-                && request in v.addSvc.requests 
-                && request.src == pkt.dest
-                && request.dest == pkt.src)
-        && (forall request: Message<AddSvc.ServiceRequest> ::
-            && request in v.addSvc.requests ==>
-            && Message(request.src, request.dest, AddSvc.MarshallServiceRequest(request.msg)) in v.network.sentMsgs)
-    }
+    lemma {:axiom} UniqueParsingAxiom(pkt: seq<byte>)
+        ensures Service.ParseServiceReply(pkt).Some? || Service.ParseServiceRequest(pkt).Some? ==> AddSvc.ParseServiceReply(pkt).None? && AddSvc.ParseServiceRequest(pkt).None?
+        ensures AddSvc.ParseServiceReply(pkt).Some? || AddSvc.ParseServiceRequest(pkt).Some? ==> Service.ParseServiceReply(pkt).None? && Service.ParseServiceRequest(pkt).None?
 
+    /// invariant tying network state to protocol state
+    // can this be generalized and baked into the system model?
     ghost predicate Inv_MultSvcCorrespondence(c: Constants, v: Variables)
         requires v.WF(c)
     {
         && (forall pkt: Message<seq<byte>> :: 
             && pkt in v.network.sentMsgs
-            && Spec.ParseServiceReply(pkt.msg).Some? ==>
-                exists request: Message<Spec.ServiceRequest> :: 
-                && Message(pkt.src, pkt.dest, Spec.ParseServiceReply(pkt.msg).value) in v.multSvc.hosts[0].replies
+            && Service.ParseServiceReply(pkt.msg).Some?
+            && pkt.src == c.multSvc.hosts[0].idSelf ==>
+                exists request: Message<Service.ServiceRequest> :: 
+                && Message(pkt.src, pkt.dest, Service.ParseServiceReply(pkt.msg).value) in v.multSvc.hosts[0].replies
                 && request in v.multSvc.hosts[0].requests 
                 && request.src == pkt.dest
                 && request.dest == pkt.src)
-        && (forall request: Message<Spec.ServiceRequest> ::
+        && (forall request: Message<Service.ServiceRequest> ::
             && request in v.multSvc.hosts[0].requests ==>
-            && Message(request.src, request.dest, Spec.MarshallServiceRequest(request.msg)) in v.network.sentMsgs)
+            && Message(request.src, request.dest, Service.MarshallServiceRequest(request.msg)) in v.network.sentMsgs
+            && request.dest == c.multSvc.hosts[0].idSelf)
     }
 
+    /// "core" invariant for protocol correctness
+    ghost predicate Inv_MultSvcInductiveMultiplication(c: Constants, v: Variables) 
+        requires v.WF(c)
+    {
+        && (forall pkt: Message<seq<byte>> ::
+            && pkt in v.network.sentMsgs
+            && AddSvc.ParseServiceRequest(pkt.msg).Some?
+            && pkt.src == c.multSvc.hosts[0].idSelf ==>
+                Inv_MultSvcInductiveMultiplicationImpl(c, v, pkt))
+    }
+
+    ghost predicate Inv_MultSvcInductiveMultiplicationImpl(c: Constants, v: Variables, pkt: Message<seq<byte>>)
+        requires v.WF(c)
+        requires pkt in v.network.sentMsgs
+        requires AddSvc.ParseServiceRequest(pkt.msg).Some?
+        requires pkt.src == c.multSvc.hosts[0].idSelf
+    {
+        var vHost := v.multSvc.hosts[0];
+        var addReq := AddSvc.ParseServiceRequest(pkt.msg).value;
+            && addReq.seqNo in vHost.seqNoAssgn
+            && addReq.x == (addReq.seqNo - vHost.firstSeqNo[vHost.seqNoAssgn[addReq.seqNo]]) * vHost.seqNoAssgn[addReq.seqNo].msg.y
+            && addReq.y == vHost.seqNoAssgn[addReq.seqNo].msg.y
+            && addReq.seqNo < vHost.nextSeqNo
+    }
+
+    /// invariant tying network state to service implementation
+    // can this be generalized and baked into the system model?
     ghost predicate Inv_AddSvcImpl(c: Constants, v: Variables)
         requires v.WF(c)
     {
         && (forall pkt: Message<seq<byte>> :: 
             && pkt in v.network.sentMsgs
-            && AddSvc.ParseServiceReply(pkt.msg).Some? ==>
-                exists request: Message<AddSvc.ServiceRequest> :: 
-                && request in v.addSvc.requests 
-                && AddSvc.ParseServiceReply(pkt.msg).value == AddSvc.AddReply(request.msg.seqNo, request.msg.x + request.msg.y))
+            && AddSvc.ParseServiceReply(pkt.msg).Some?
+            && pkt.src == c.addSvc.idSelf ==>
+                exists req_pkt: Message<seq<byte>> :: 
+                && req_pkt in v.network.sentMsgs
+                && AddSvc.ParseServiceRequest(req_pkt.msg).Some?
+                && AddSvc.ParseServiceReply(pkt.msg).value.seqNo == AddSvc.ParseServiceRequest(req_pkt.msg).value.seqNo
+                && AddSvc.ParseServiceReply(pkt.msg).value.sum == AddSvc.ParseServiceRequest(req_pkt.msg).value.x + AddSvc.ParseServiceRequest(req_pkt.msg).value.y
+                && pkt.src == req_pkt.dest
+                && pkt.dest == req_pkt.src
+        )
     }
 
     ghost predicate Inv(c: Constants, v: Variables)
     {
         && v.WF(c)
-        && Inv_AddSvcCorrespondence(c, v)
         && Inv_MultSvcCorrespondence(c, v)
+        && Inv_MultSvcInductiveMultiplication(c, v)
+        && Inv_AddSvcImpl(c, v)
     }
 
     lemma RefinementInit(c: Constants, v: Variables)
         // requires Init(c, v)
         // ensures Inv(c, v)
-        // ensures Spec.Init(ConstantsAbstraction(c), VariablesAbstraction(c, v))
+        // ensures Service.Init(ConstantsAbstraction(c), VariablesAbstraction(c, v))
     {}
+
+    lemma InvInductive_ReceiveRequestHelper(c: Constants, v: Variables, v': Variables, msgOps: MessageOps, request: Message<Service.ServiceRequest>)
+        requires Next(c, v, v', msgOps)
+        requires Inv(c, v)
+        requires MultSvc.Host.ReceiveRequestImpl(c.multSvc.hosts[0], v.multSvc.hosts[0], v'.multSvc.hosts[0], msgOps, request)
+        ensures Inv(c, v')
+    {
+        var cHost := c.multSvc.hosts[0];
+        var vHost := v.multSvc.hosts[0];
+        var v'Host := v'.multSvc.hosts[0];
+        assert msgOps.recv == {Message(request.src, request.dest, Service.MarshallServiceRequest(request.msg))};
+        var sent :| msgOps.send == {sent};
+        var addReq := AddSvc.AddRequest(vHost.nextSeqNo, 0, request.msg.y);
+        assert sent == Message(cHost.idSelf, cHost.idAdditionService, AddSvc.MarshallServiceRequest(addReq));
+        UniqueParsingAxiom(sent.msg);
+        AddSvc.ParseMarshallServiceRequestInverse(addReq);
+        assert Inv_MultSvcCorrespondence(c, v');
+        assert Inv_AddSvcImpl(c, v');
+
+        assert v'.network.sentMsgs == v.network.sentMsgs + {sent};
+        assert AddSvc.ParseServiceRequest(sent.msg).Some?;
+        assert addReq == AddSvc.ParseServiceRequest(sent.msg).value;
+        assert addReq.seqNo == vHost.nextSeqNo;
+        assert v'Host.firstSeqNo[request] == vHost.nextSeqNo;
+        assert v'Host.seqNoAssgn[vHost.nextSeqNo] == request;
+        assert addReq.seqNo == v'Host.firstSeqNo[v'Host.seqNoAssgn[addReq.seqNo]];
+        assert addReq.x == 0;
+        assert addReq.y == request.msg.y;
+        forall pkt | pkt in v'.network.sentMsgs && AddSvc.ParseServiceRequest(pkt.msg).Some? && pkt.src == c.multSvc.hosts[0].idSelf
+            ensures Inv_MultSvcInductiveMultiplicationImpl(c, v', pkt)
+        {
+            if (pkt == sent) {
+                assert Inv_MultSvcInductiveMultiplicationImpl(c, v', pkt);
+            } else {
+                assert pkt in v.network.sentMsgs;
+                assert Inv_MultSvcInductiveMultiplication(c, v);
+                var addReq := AddSvc.ParseServiceRequest(pkt.msg).value;
+                assert addReq.seqNo in v'Host.seqNoAssgn;
+                assert vHost.seqNoAssgn[addReq.seqNo] == v'Host.seqNoAssgn[addReq.seqNo];
+                assert vHost.firstSeqNo[vHost.seqNoAssgn[addReq.seqNo]] == v'Host.firstSeqNo[v'Host.seqNoAssgn[addReq.seqNo]];
+                assert vHost.nextSeqNo < v'Host.nextSeqNo;
+                assert Inv_MultSvcInductiveMultiplicationImpl(c, v', pkt);
+            }
+        }
+        assert Inv_MultSvcInductiveMultiplication(c, v');
+    }
+
+    lemma InductiveMultiplicationHelper(a: int, b: int, p: int)
+        requires a * b + b == p
+        ensures (a + 1) * b == p
+    {}
+
+    lemma InvInductive_ReceiveIntermediateResponseHelper(c: Constants, v: Variables, v': Variables, msgOps: MessageOps, svcReply: Message<AddSvc.ServiceReply>) 
+        requires Next(c, v, v', msgOps)
+        requires Inv(c, v)
+        requires MultSvc.Host.ReceiveIntermediateResponseImpl(c.multSvc.hosts[0], v.multSvc.hosts[0], v'.multSvc.hosts[0], msgOps, svcReply)
+        ensures Inv(c, v')
+    {
+        var cHost := c.multSvc.hosts[0];
+        var vHost := v.multSvc.hosts[0];
+        var v'Host := v'.multSvc.hosts[0];
+        assert msgOps.recv == {Message(svcReply.src, svcReply.dest, AddSvc.MarshallServiceReply(svcReply.msg))};
+        var sent :| msgOps.send == {sent};
+        var addReq := AddSvc.AddRequest(svcReply.msg.seqNo + 1, svcReply.msg.sum, vHost.seqNoAssgn[svcReply.msg.seqNo].msg.y);
+        assert sent == Message(cHost.idSelf, cHost.idAdditionService, AddSvc.MarshallServiceRequest(addReq));
+        UniqueParsingAxiom(sent.msg);
+        AddSvc.ParseMarshallServiceRequestInverse(addReq);
+        assert Inv_MultSvcCorrespondence(c, v');
+        assert Inv_AddSvcImpl(c, v');
+
+        assert v'.network.sentMsgs == v.network.sentMsgs + {sent};
+        assert AddSvc.ParseServiceRequest(sent.msg).Some?;
+        assert addReq == AddSvc.ParseServiceRequest(sent.msg).value;
+        assert addReq.seqNo == svcReply.msg.seqNo + 1;
+        var request := vHost.seqNoAssgn[svcReply.msg.seqNo];
+        assert svcReply.msg.seqNo == vHost.firstSeqNo[request] + |vHost.intermediateResults[request]|;
+        assert addReq.x == svcReply.msg.sum;
+        assert addReq.y == request.msg.y;
+        forall pkt | pkt in v'.network.sentMsgs && AddSvc.ParseServiceRequest(pkt.msg).Some? && pkt.src == c.multSvc.hosts[0].idSelf
+            ensures Inv_MultSvcInductiveMultiplicationImpl(c, v', pkt)
+        {
+            if (pkt == sent) {
+                assert Inv_MultSvcInductiveMultiplication(c, v);
+                var prevAddResp :| msgOps.recv == {prevAddResp};
+                assert prevAddResp.msg == AddSvc.MarshallServiceReply(svcReply.msg);
+                AddSvc.MarshallParseInverse(prevAddResp.msg);
+                assert AddSvc.ParseServiceReply(prevAddResp.msg).Some?;
+                assert prevAddResp.src == c.addSvc.idSelf;
+                var prevAddReq :| prevAddReq in v.network.sentMsgs && AddSvc.ParseServiceRequest(prevAddReq.msg).Some? && AddSvc.ParseServiceReply(prevAddResp.msg).value.seqNo == AddSvc.ParseServiceRequest(prevAddReq.msg).value.seqNo && AddSvc.ParseServiceReply(prevAddResp.msg).value.sum == AddSvc.ParseServiceRequest(prevAddReq.msg).value.x + AddSvc.ParseServiceRequest(prevAddReq.msg).value.y && prevAddResp.src == prevAddReq.dest && prevAddResp.dest == prevAddReq.src;
+                assert prevAddReq.src == c.multSvc.hosts[0].idSelf;
+                assert Inv_MultSvcInductiveMultiplicationImpl(c, v, prevAddReq);
+                var prevAddReqParsed := AddSvc.ParseServiceRequest(prevAddReq.msg).value;
+                AddSvc.ParseMarshallServiceReplyInverse(svcReply.msg);
+                assert prevAddReqParsed.seqNo == svcReply.msg.seqNo;
+                assert prevAddReqParsed.seqNo + 1 == addReq.seqNo;
+                assert prevAddReqParsed.x == (prevAddReqParsed.seqNo - vHost.firstSeqNo[vHost.seqNoAssgn[prevAddReqParsed.seqNo]]) * vHost.seqNoAssgn[prevAddReqParsed.seqNo].msg.y && prevAddReqParsed.y == vHost.seqNoAssgn[prevAddReqParsed.seqNo].msg.y;
+                AddSvc.ParseMarshallServiceReplyInverse(svcReply.msg);
+                assert svcReply.msg.sum == (prevAddReqParsed.seqNo - vHost.firstSeqNo[vHost.seqNoAssgn[prevAddReqParsed.seqNo]]) * vHost.seqNoAssgn[prevAddReqParsed.seqNo].msg.y + vHost.seqNoAssgn[prevAddReqParsed.seqNo].msg.y;
+                InductiveMultiplicationHelper(prevAddReqParsed.seqNo - vHost.firstSeqNo[vHost.seqNoAssgn[prevAddReqParsed.seqNo]], vHost.seqNoAssgn[prevAddReqParsed.seqNo].msg.y, svcReply.msg.sum);
+                assert addReq.x == (addReq.seqNo - v'Host.firstSeqNo[vHost.seqNoAssgn[addReq.seqNo]]) * v'Host.seqNoAssgn[addReq.seqNo].msg.y;
+                assert addReq.y ==  v'Host.seqNoAssgn[addReq.seqNo].msg.y;
+                assert addReq.seqNo in v'Host.seqNoAssgn;
+                assert addReq.seqNo < v'Host.nextSeqNo;
+                assert Inv_MultSvcInductiveMultiplicationImpl(c, v', pkt);
+            } else {
+                assert pkt in v.network.sentMsgs;
+                assert Inv_MultSvcInductiveMultiplication(c, v);
+                var addReq := AddSvc.ParseServiceRequest(pkt.msg).value;
+                assert addReq.seqNo in v'Host.seqNoAssgn;
+                assert vHost.seqNoAssgn[addReq.seqNo] == v'Host.seqNoAssgn[addReq.seqNo];
+                assert vHost.firstSeqNo[vHost.seqNoAssgn[addReq.seqNo]] == v'Host.firstSeqNo[v'Host.seqNoAssgn[addReq.seqNo]];
+            }
+        }
+        assert Inv_MultSvcInductiveMultiplication(c, v');
+    }
+
+    lemma InvInductive_ReceiveFinalResponseHelper(c: Constants, v: Variables, v': Variables, msgOps: MessageOps, svcReply: Message<AddSvc.ServiceReply>) 
+        requires Next(c, v, v', msgOps)
+        requires Inv(c, v)
+        requires MultSvc.Host.ReceiveFinalResponseImpl(c.multSvc.hosts[0], v.multSvc.hosts[0], v'.multSvc.hosts[0], msgOps, svcReply)
+        ensures Inv(c, v')
+    {
+        var cHost := c.multSvc.hosts[0];
+        var vHost := v.multSvc.hosts[0];
+        var v'Host := v'.multSvc.hosts[0];
+
+        var svcReply :| MultSvc.Host.ReceiveFinalResponseImpl(cHost, vHost, v'Host, msgOps, svcReply);
+        assert msgOps.recv == {Message(svcReply.src, svcReply.dest, AddSvc.MarshallServiceReply(svcReply.msg))};
+        var sent :| msgOps.send == {sent};
+        var multSvcReply := Service.MultiplyReply(vHost.seqNoAssgn[svcReply.msg.seqNo].msg.seqNo, svcReply.msg.sum);
+        assert sent == Message(cHost.idSelf, vHost.seqNoAssgn[svcReply.msg.seqNo].src, Service.MarshallServiceReply(multSvcReply));
+        Service.MarshallParseInverse(sent.msg);
+        assert Service.ParseServiceReply(sent.msg).Some?;
+        Service.ParseMarshallServiceReplyInverse(multSvcReply);
+        assert multSvcReply == Service.ParseServiceReply(sent.msg).value;
+        var request := vHost.seqNoAssgn[svcReply.msg.seqNo];
+        assert request in vHost.requests;
+        assert request.src == sent.dest && request.dest == sent.src;
+        assert Inv_MultSvcCorrespondence(c, v');
+        assert Inv_AddSvcImpl(c, v');
+
+        UniqueParsingAxiom(sent.msg);
+        assert Inv_MultSvcInductiveMultiplication(c, v');
+    }
+
+    lemma InvInductive(c: Constants, v: Variables, v': Variables, msgOps: MessageOps) 
+        requires Next(c, v, v', msgOps)
+        requires Inv(c, v)
+        ensures Inv(c, v') 
+    {
+        var step :| NextStep(c, v, v', msgOps, step);
+        if (MultSvcAction(c, v, v', msgOps, step.hostId)) {
+            var hostStep :| MultSvc.NextStep(c.multSvc, v.multSvc, v'.multSvc, msgOps, hostStep);
+            var cHost := c.multSvc.hosts[0];
+            var vHost := v.multSvc.hosts[0];
+            var v'Host := v'.multSvc.hosts[0];
+            assert MultSvc.Host.Next(cHost, vHost, v'Host, msgOps);
+
+            if (MultSvc.Host.ReceiveRequest(cHost, vHost, v'Host, msgOps)) {
+                var request :| MultSvc.Host.ReceiveRequestImpl(cHost, vHost, v'Host, msgOps, request);
+                InvInductive_ReceiveRequestHelper(c, v, v', msgOps, request);
+            } else if (MultSvc.Host.ReceiveIntermediateResponse(cHost, vHost, v'Host, msgOps)) {
+                var svcReply :| MultSvc.Host.ReceiveIntermediateResponseImpl(cHost, vHost, v'Host, msgOps, svcReply);
+                InvInductive_ReceiveIntermediateResponseHelper(c, v, v', msgOps, svcReply);
+            } else {
+                assert MultSvc.Host.ReceiveFinalResponse(cHost, vHost, v'Host, msgOps);
+                var svcReply :| MultSvc.Host.ReceiveFinalResponseImpl(cHost, vHost, v'Host, msgOps, svcReply);
+                InvInductive_ReceiveFinalResponseHelper(c, v, v', msgOps, svcReply);
+            }
+        } else {
+            assert AddSvcAction(c, v, v', msgOps, step.hostId);
+            var sent :| msgOps.send == {sent};
+            var request: Message<AddSvc.ServiceRequest>, reply: Message<AddSvc.ServiceReply> :| msgOps.recv == {Message(request.src, request.dest, AddSvc.MarshallServiceRequest(request.msg))} && msgOps.send == {Message(reply.src, reply.dest, AddSvc.MarshallServiceReply(reply.msg))} && reply.msg == AddSvc.AddReply(request.msg.seqNo, request.msg.x + request.msg.y) && reply.dest == request.src;
+            assert sent == Message(reply.src, reply.dest, AddSvc.MarshallServiceReply(reply.msg));
+            AddSvc.MarshallParseInverse(sent.msg);
+            assert AddSvc.ParseServiceReply(sent.msg).Some?;
+            var recv :| msgOps.recv == {recv};
+            assert recv == Message(request.src, request.dest, AddSvc.MarshallServiceRequest(request.msg));
+            AddSvc.MarshallParseInverse(recv.msg); 
+            assert AddSvc.ParseServiceRequest(recv.msg).Some?;
+
+            assert Inv_MultSvcCorrespondence(c, v');
+            
+            forall pkt: Message<seq<byte>> | pkt in v'.network.sentMsgs && AddSvc.ParseServiceReply(pkt.msg).Some? && pkt.src == c.addSvc.idSelf
+                ensures (exists req_pkt: Message<seq<byte>> :: 
+                && req_pkt in v.network.sentMsgs
+                && AddSvc.ParseServiceRequest(req_pkt.msg).Some?
+                && AddSvc.ParseServiceReply(pkt.msg).value.seqNo == AddSvc.ParseServiceRequest(req_pkt.msg).value.seqNo
+                && AddSvc.ParseServiceReply(pkt.msg).value.sum == AddSvc.ParseServiceRequest(req_pkt.msg).value.x + AddSvc.ParseServiceRequest(req_pkt.msg).value.y
+                && pkt.src == req_pkt.dest
+                && pkt.dest == req_pkt.src)
+            {
+                if (pkt == sent) {
+                    assert recv in v'.network.sentMsgs;
+                    AddSvc.ParseMarshallServiceReplyInverse(reply.msg);
+                    AddSvc.ParseMarshallServiceRequestInverse(request.msg);
+                    assert AddSvc.ParseServiceRequest(recv.msg).Some? && AddSvc.ParseServiceReply(pkt.msg).value.seqNo == AddSvc.ParseServiceRequest(recv.msg).value.seqNo && AddSvc.ParseServiceReply(pkt.msg).value.sum == AddSvc.ParseServiceRequest(recv.msg).value.x + AddSvc.ParseServiceRequest(recv.msg).value.y;
+                } else {
+                    assert pkt in v.network.sentMsgs;
+                }
+            }
+            assert Inv_AddSvcImpl(c, v');
+            assert v.multSvc.hosts[0] == v'.multSvc.hosts[0];
+            assert Inv_MultSvcInductiveMultiplication(c, v');
+        }
+    }
     
+    /*
     lemma RefinementNext(c: Constants, v: Variables, v': Variables, msgOps: MessageOps)
         // requires Next(c, v, v', msgOps)
         // requires Inv(c, v)
         // ensures Inv(c, v') 
         // ensures 
-        //     || Spec.Next(ConstantsAbstraction(c), VariablesAbstraction(c, v), VariablesAbstraction(c, v'), MessageOps(ServiceRequestsAbstraction(msgOps.recv), ServiceRepliesAbstraction(msgOps.send)))
+        //     || Service.Next(ConstantsAbstraction(c), VariablesAbstraction(c, v), VariablesAbstraction(c, v'), MessageOps(ServiceRequestsAbstraction(msgOps.recv), ServiceRepliesAbstraction(msgOps.send)))
         //     || (VariablesAbstraction(c, v) == VariablesAbstraction(c, v') && ServiceRequestsAbstraction(msgOps.recv) == {} && ServiceRepliesAbstraction(msgOps.send) == {})
     {
-        if (Spec.Next(ConstantsAbstraction(c), VariablesAbstraction(c, v), VariablesAbstraction(c, v'), MessageOps(ServiceRequestsAbstraction(msgOps.recv), ServiceRepliesAbstraction(msgOps.send)))) {
-
-        }
-        else {
+        var step :| NextStep(c, v, v', msgOps, step);
+        if (MultSvcAction(c, v, v', msgOps, step.hostId)) {
+            InvInductive(c, v, v', msgOps);
             assume false;
+        } else {
+            InvInductive(c, v, v', msgOps);   
+            assume false;         
         }
     }
+    */
 
 }
