working/composition/event_based_refinement/load_balancer/service_correspondence/shared/RefinementObligation.t.dfy
@@ -1,22 +1,22 @@
 include "AbstractDistributedComponent.t.dfy"
 
 abstract module RefinementTheorem refines AbstractDistributedComponent {
-    ghost function ConstantsAbstraction(c: Constants) : Host.Spec.Constants
+    ghost function ConstantsAbstraction(c: Constants) : Host.Service.Constants
         requires c.WF()
 
-    ghost function VariablesAbstraction(c: Constants, v: Variables) : Host.Spec.Variables
+    ghost function VariablesAbstraction(c: Constants, v: Variables) : Host.Service.Variables
         requires v.WF(c)
 
     ghost function ServiceRequestsAbstraction(pkts: set<Message<seq<byte>>>) : set<Message<seq<byte>>>
-        ensures forall bytes :: bytes in pkts && Host.Spec.ParseServiceRequest(bytes.msg).Some? ==> bytes in ServiceRequestsAbstraction(pkts)
-        ensures forall m :: m in ServiceRequestsAbstraction(pkts) ==> exists bytes :: bytes in pkts && Host.Spec.ParseServiceRequest(bytes.msg).Some? && m == bytes
+        ensures forall bytes :: bytes in pkts && Host.Service.ParseServiceRequest(bytes.msg).Some? ==> bytes in ServiceRequestsAbstraction(pkts)
+        ensures forall m :: m in ServiceRequestsAbstraction(pkts) ==> exists bytes :: bytes in pkts && Host.Service.ParseServiceRequest(bytes.msg).Some? && m == bytes
     {
         if (pkts == {}) then 
             {}
         else 
             assert exists bytes :: bytes in pkts;
             var bytes :| bytes in pkts;
-            var req := Host.Spec.ParseServiceRequest(bytes.msg);
+            var req := Host.Service.ParseServiceRequest(bytes.msg);
             if (req != None) then
                 {bytes} + ServiceRequestsAbstraction(pkts - {bytes})
             else
@@ -25,30 +25,30 @@ abstract module RefinementTheorem refines AbstractDistributedComponent {
 
 
     lemma ServiceRequestsAbstractionLemma(pkts: set<Message<seq<byte>>>)
-        ensures forall m : Message<seq<byte>> :: m in pkts && Host.Spec.ParseServiceRequest(m.msg).Some? <==> m in ServiceRequestsAbstraction(pkts)
+        ensures forall m : Message<seq<byte>> :: m in pkts && Host.Service.ParseServiceRequest(m.msg).Some? <==> m in ServiceRequestsAbstraction(pkts)
     {
-        forall m : Message<seq<byte>> | m in pkts && Host.Spec.ParseServiceRequest(m.msg).Some?
+        forall m : Message<seq<byte>> | m in pkts && Host.Service.ParseServiceRequest(m.msg).Some?
             ensures m in ServiceRequestsAbstraction(pkts)
         {
             assert m in ServiceRequestsAbstraction(pkts);
         }
         forall m : Message<seq<byte>> | m in ServiceRequestsAbstraction(pkts) 
-            ensures m in pkts && Host.Spec.ParseServiceRequest(m.msg).Some?
+            ensures m in pkts && Host.Service.ParseServiceRequest(m.msg).Some?
         {
-            var bytes :| bytes in pkts && Host.Spec.ParseServiceRequest(bytes.msg).Some? && m == bytes;
+            var bytes :| bytes in pkts && Host.Service.ParseServiceRequest(bytes.msg).Some? && m == bytes;
         }
     }
 
     ghost function ServiceRepliesAbstraction(pkts: set<Message<seq<byte>>>) : set<Message<seq<byte>>>
-        ensures forall bytes :: bytes in pkts && Host.Spec.ParseServiceReply(bytes.msg).Some? ==> bytes in ServiceRepliesAbstraction(pkts)
-        ensures forall m :: m in ServiceRepliesAbstraction(pkts) ==> exists bytes :: bytes in pkts && Host.Spec.ParseServiceReply(bytes.msg).Some? && m == bytes
+        ensures forall bytes :: bytes in pkts && Host.Service.ParseServiceReply(bytes.msg).Some? ==> bytes in ServiceRepliesAbstraction(pkts)
+        ensures forall m :: m in ServiceRepliesAbstraction(pkts) ==> exists bytes :: bytes in pkts && Host.Service.ParseServiceReply(bytes.msg).Some? && m == bytes
     {
         if (pkts == {}) then 
             {}
         else 
             assert exists bytes :: bytes in pkts;
             var bytes :| bytes in pkts;
-            var req := Host.Spec.ParseServiceReply(bytes.msg);
+            var req := Host.Service.ParseServiceReply(bytes.msg);
             if (req != None) then
                 {bytes} + ServiceRepliesAbstraction(pkts - {bytes})
             else
@@ -56,9 +56,9 @@ abstract module RefinementTheorem refines AbstractDistributedComponent {
     }
 
     lemma ServiceRepliesAbstractionLemma(pkts: set<Message<seq<byte>>>)
-        ensures forall m : Message<seq<byte>> :: m in pkts && Host.Spec.ParseServiceReply(m.msg).Some? <==> m in ServiceRepliesAbstraction(pkts)
+        ensures forall m : Message<seq<byte>> :: m in pkts && Host.Service.ParseServiceReply(m.msg).Some? <==> m in ServiceRepliesAbstraction(pkts)
     {
-        forall m : Message<seq<byte>> | m in pkts && Host.Spec.ParseServiceReply(m.msg).Some?
+        forall m : Message<seq<byte>> | m in pkts && Host.Service.ParseServiceReply(m.msg).Some?
             ensures m in ServiceRepliesAbstraction(pkts)
         {
             assert m in ServiceRepliesAbstraction(pkts);
@@ -66,7 +66,7 @@ abstract module RefinementTheorem refines AbstractDistributedComponent {
         forall m : Message<seq<byte>> | m in ServiceRepliesAbstraction(pkts) 
             ensures m in pkts
         {
-            var bytes :| bytes in pkts && Host.Spec.ParseServiceReply(bytes.msg).Some? && m == bytes;
+            var bytes :| bytes in pkts && Host.Service.ParseServiceReply(bytes.msg).Some? && m == bytes;
         }
     }
 
@@ -75,13 +75,13 @@ abstract module RefinementTheorem refines AbstractDistributedComponent {
     lemma RefinementInit(c: Constants, v: Variables)
         requires Init(c, v)
         ensures Inv(c, v)
-        ensures Host.Spec.Init(ConstantsAbstraction(c), VariablesAbstraction(c, v))
+        ensures Host.Service.Init(ConstantsAbstraction(c), VariablesAbstraction(c, v))
     
     lemma RefinementNext(c: Constants, v: Variables, v': Variables, msgOps: MessageOps)
         requires Next(c, v, v', msgOps)
         requires Inv(c, v)
         ensures Inv(c, v') 
         ensures 
-            || Host.Spec.Next(ConstantsAbstraction(c), VariablesAbstraction(c, v), VariablesAbstraction(c, v'), MessageOps(ServiceRequestsAbstraction(msgOps.recv), ServiceRepliesAbstraction(msgOps.send)))
+            || Host.Service.Next(ConstantsAbstraction(c), VariablesAbstraction(c, v), VariablesAbstraction(c, v'), MessageOps(ServiceRequestsAbstraction(msgOps.recv), ServiceRepliesAbstraction(msgOps.send)))
             || (VariablesAbstraction(c, v) == VariablesAbstraction(c, v') && ServiceRequestsAbstraction(msgOps.recv) == {} && ServiceRepliesAbstraction(msgOps.send) == {})
 }
