working/composition/event_based_refinement/load_balancer/service_correspondence/shared/AbstractServiceSM.t.dfy
@@ -1,0 +1,31 @@
+include "Types.t.dfy"
+
+abstract module AbstractServiceSM {
+    import opened Types
+
+    type ServiceRequest
+    type ServiceReply
+
+    type Constants
+    type Variables
+
+    ghost predicate Init(c: Constants, v: Variables)
+    ghost predicate Next(c: Constants, v: Variables, v': Variables, msgOps: MessageOps)
+
+    ghost function MarshallServiceRequest(request: ServiceRequest): seq<byte>
+    ghost function MarshallServiceReply(reply: ServiceReply): seq<byte>
+    ghost function ParseServiceRequest(bytes: seq<byte>): Option<ServiceRequest>
+    ghost function ParseServiceReply(bytes: seq<byte>): Option<ServiceReply>
+    
+    lemma MarshallParseInverse(bytes: seq<byte>)
+        ensures ParseServiceRequest(bytes).Some? ==> MarshallServiceRequest(ParseServiceRequest(bytes).value) == bytes
+        ensures ParseServiceReply(bytes).Some? ==> MarshallServiceReply(ParseServiceReply(bytes).value) == bytes
+        ensures forall req :: bytes == MarshallServiceRequest(req) ==> ParseServiceRequest(bytes).Some?
+        ensures forall repl :: bytes == MarshallServiceReply(repl) ==> ParseServiceReply(bytes).Some?
+
+    lemma ParseMarshallServiceRequestInverse(req: ServiceRequest)
+        ensures ParseServiceRequest(MarshallServiceRequest(req)).Some? && ParseServiceRequest(MarshallServiceRequest(req)).value == req
+
+    lemma ParseMarshallServiceReplyInverse(repl: ServiceReply)
+        ensures ParseServiceReply(MarshallServiceReply(repl)).Some? && ParseServiceReply(MarshallServiceReply(repl)).value == repl
+}
